src/missing.lean
@@ -3,19 +3,30 @@ import data.list.indexes
 import data.list.nodup
 import data.list.range
 
+lemma list.find_indexes_nth_nmem {α : Type*} {l : list α} {n : ℕ} {p : α → Prop} [decidable_pred p] :
+  ∀ {x}, l.nth n = some x → ¬(p x) → n ∉ (l.find_indexes p) :=
+  sorry
+
+lemma list.find_indexes_nth_none {α : Type*} {l : list α} {n : ℕ} {p : α → Prop} [decidable_pred p] :
+  l.nth n = none → n ∉ (l.find_indexes p) :=
+  sorry
+
+-- https://leanprover.zulipchat.com/#narrow/stream/217875-Is-there.20code.20for.20X.3F/topic/list.2Enth.20is.20either.20none/near/226562824
+lemma option.join_eq_none {α : Type*} (o : option (option α)) : o.join = none ↔ o = none ∨ o = some none :=
+  by rcases o with _|_|_; simp
+
 -- https://leanprover.zulipchat.com/#narrow/stream/217875-Is-there.20code.20for.20X.3F/topic/list.2Eupdate_nth_comm/near/223010209
 @[simp]
-lemma list.update_nth_nil (α : Type) (n : ℕ) (a : α) : [].update_nth n a = [] := rfl
-lemma list.update_nth_comm (α : Type) (a b : α) : Π (n m : ℕ) (h : n ≠ m) (l : list α),
-  (l.update_nth n a).update_nth m b =
-  (l.update_nth m b).update_nth n a
+lemma list.update_nth_nil {α : Type*} (n : ℕ) (a : α) : [].update_nth n a = [] := rfl
+lemma list.update_nth_comm {α : Type*} (a b : α) : ∀ {n m : ℕ} (h : n ≠ m) (l : list α),
+  (l.update_nth n a).update_nth m b = (l.update_nth m b).update_nth n a
   | _ _ _ [] := by simp
   | 0 0 h (x :: t) := absurd rfl h
   | (n + 1) 0 h (x :: t) := by simp [list.update_nth]
   | 0 (m + 1) h (x :: t) := by simp [list.update_nth]
-  | (n + 1) (m + 1) h (x :: t) := by { simp [list.update_nth], exact list.update_nth_comm n m (λ h', h $ nat.succ_inj'.mpr h') t}
+  | (n + 1) (m + 1) h (x :: t) := by { simp [list.update_nth], exact list.update_nth_comm (λ h', h $ nat.succ_inj'.mpr h') t}
 
--- Courtesy of Yakov Pechersky: https://leanprover.zulipchat.com/#narrow/stream/113489-new-members/topic/Nodup.20Indices/near/224749989
+-- https://leanprover.zulipchat.com/#narrow/stream/113489-new-members/topic/Nodup.20Indices/near/224749989
 
 open list
 
