src/precedence/basic.lean
@@ -109,7 +109,7 @@ namespace precedence.graph
 
   -- If two reactions `i` and `i'` are independent, then none of `i`'s antidependencies (output ports)
   -- have a connection any of `i'`'s dependencies (input ports).
-  lemma indep_rcns_no_edge {η : network.graph υ} {ρ : precedence.graph υ} (h : ρ.is_well_formed_over η) {i i' : reaction.id} :
+  lemma indep_rcns_not_ext_dep {η : network.graph υ} {ρ : precedence.graph υ} (h : ρ.is_well_formed_over η) {i i' : reaction.id} :
     i ≠ i' → ¬(i~ρ~>i') → ¬(externally_dependent i i' η) :=
     begin 
       intros hₙ hₚ,
